day 5

problems/5/Problem5.dfy
@@ -1,9 +1,153 @@
+include "../../parser/split.dfy"
+include "../../parser/parseInt.dfy"
 module Problem5 {
-    method problem5_1(input: string) returns (x: int) {
-        return 3;
+    import opened Split
+    import opened ParseInt
+    import opened Std.Collections.Seq
+    import opened Std.Relations
+
+    method parseInput(input: string) returns (ranges: seq<(nat,nat)>, ids: seq<nat>)
+        ensures forall range :: range in ranges ==> range.0 <= range.1
+    {
+        var pieces := splitOnDoubleBreak(input);
+        expect |pieces| == 2;
+        // print "pieces 0 ", pieces[0];
+        var rangeStrings := splitOnBreak(pieces[0]);
+        var idStrings := splitOnBreak(pieces[1]);
+
+        ranges := [];
+        ids := [];
+        for i := 0 to |rangeStrings| 
+            invariant |ranges| == i
+            invariant forall range :: range in ranges ==> range.0 <= range.1
+        {
+            var split_range := split(rangeStrings[i], "-");
+            // print "\n", split_range;
+            expect |split_range| == 2;
+            var start := Integer(split_range[0]);
+            var end := Integer(split_range[1]);
+            // print "\ns ", start, " ",  end; 
+            expect 0 < start <= end;
+            ranges := ranges + [(start, end)];
+        }
+
+        for i := 0 to |idStrings|
+            invariant |ids| == i
+        {
+            var id := Integer(idStrings[i]);
+            expect 0 < id;
+            ids := ids + [id];
+        }
     }
 
-    method problem5_2(input: string) returns (x: int) {
-        return 4;
+    predicate IsFresh(range: (nat, nat), id: nat) {
+        range.0 <= id <= range.1
+    }
+
+    predicate IsInRanges(ranges: seq<(nat,nat)>, id: nat) {
+        exists i :: 0 <= i < |ranges| && IsFresh(ranges[i], id)
+    }
+
+    //fresh count function
+    method problem5_1(input: string) returns (answer: int) {
+        var ranges, ids := parseInput(input);
+        answer := 0;
+        for i := 0 to |ids| 
+        {
+            if IsInRanges(ranges, ids[i]) {
+                answer := answer + 1;
+            }
+        }
+        print "\n";
+    }
+
+    predicate IsOverlapping(left: (nat, nat), right: (nat,nat)) {
+        !(left.1 < right.0 || right.1 < left.0)
+    }
+
+    lemma test() {
+        assert IsOverlapping((3,6),(6,10));
+        assert IsOverlapping((6,6),(6,10));
+        assert IsOverlapping((6,6),(5,10));
+        assert IsOverlapping((6,7),(3,10));
+        assert IsOverlapping((542009870509829, 542009870509829), (536745635162015, 542009870509829));
+        // assert IsOverlapping((3,5),(6,10));
+        // assert IsOverlapping((13,65),(6,10));
+        assert mergeRange((6,6),(6,10)) == (6,10);
+        assert mergeRange((6,7),(3,10)) == (3,10);
+    }
+
+    function min(a: nat ,b:nat): nat {
+        if a < b then a else b
+    }
+
+    function max(a: nat, b: nat): nat {
+        if a <= b then b else a
+    }
+
+    function mergeRange(left: (nat, nat), right: (nat,nat)): (nat, nat) {
+        (min(left.0, right.0), max(left.1, right.1))
+    }
+
+    predicate lteRange(left: (nat, nat), right: (nat, nat)) {
+        left.1 <= right.1
+    }
+
+    lemma {:axiom} IsTotalOrder()
+        ensures TotalOrdering(lteRange)
+
+    predicate HasOverlapping(ranges: seq<(nat,nat)>) {
+        exists i :: 0 <= i < |ranges|-1 && IsOverlapping(ranges[i], ranges[i+1])
+        // exists i, j :: 0 <= i < j < |ranges| && IsOverlapping(ranges[i], ranges[j])
+    }
+
+    function rangeSize(r: (nat,nat)): nat 
+        requires r.0<=r.1
+    {
+        (r.1-r.0)+1
+    }
+
+    function rangeSet(r: (nat, nat)): set<nat>
+        requires r.0 <= r.1
+    {
+        set x | r.0 <= x <= r.1
+    }
+
+    lemma RangeSizeEqual(r: (nat, nat))
+        requires r.0 <= r.1
+        decreases r.1 - r.0
+        ensures rangeSize(r) == |rangeSet(r)|
+    {
+        if r.0 == r.1 {
+            var s := rangeSet(r);
+            assert s == {r.0};
+        }else{
+            RangeSizeEqual((r.0, r.1-1));
+            var s := rangeSet(r);
+            assert s == rangeSet((r.0, r.1-1)) + {r.1};
+        }
+    }
+
+    method problem5_2(input: string) returns (answer: int)
+        decreases *
+    {
+        var ranges, ids := parseInput(input);
+        answer := 0;
+        IsTotalOrder();
+        var sortedRanges := MergeSortBy(lteRange, ranges);
+        assert forall r :: r in sortedRanges ==> r in multiset(sortedRanges);
+        var i := 0;
+        while HasOverlapping(sortedRanges) 
+            decreases *
+            invariant forall r :: r in sortedRanges ==> r.0 <= r.1
+        {
+            var i :| 0 <= i < |sortedRanges|-1 && IsOverlapping(sortedRanges[i], sortedRanges[i+1]);
+            sortedRanges := sortedRanges[0..i]+[mergeRange(sortedRanges[i], sortedRanges[i+1])] + sortedRanges[i+2..];
+        }
+        for i := 0 to |sortedRanges| 
+        {
+            answer := answer + rangeSize(sortedRanges[i]);
+        }
+        print "\n";
     }
 }
